floyd/globals_lemmas.v
@@ -50,13 +50,13 @@ Proof.
 Qed.
 
 Lemma tc_globalvar_sound:
-  forall Delta i t gv idata rho,
+  forall Delta i t gz idata rho,
    (var_types Delta) ! i = None ->
    (glob_types Delta) ! i = Some t ->
-   gvar_volatile gv = false ->
-   gvar_init gv = idata ->
+   gvar_volatile gz = false ->
+   gvar_init gz = idata ->
    tc_environ Delta rho ->
-   globvar2pred(i, gv) rho |-- init_data_list2pred idata (readonly2share (gvar_readonly gv)) (eval_var i t rho) rho.
+   globvar2pred (globals_of_env rho) (i, gz) rho |-- init_data_list2pred idata (readonly2share (gvar_readonly gz)) (eval_var i t rho) rho.
 Proof.
 pose (H2:=True).
 pose (H4:=True).
@@ -66,6 +66,7 @@ simpl.
 destruct H6 as [? [? [? ?]]].
 destruct (H9 i _ H0); [ | destruct H10; congruence].
 destruct (H8 _ _ H0) as [b ?].
+unfold globals_of_env. 
 rewrite H11. rewrite H1.
 rewrite H3; simpl.
 unfold eval_var.
@@ -80,8 +81,8 @@ Lemma tc_globalvar_sound':
    gvar_volatile gv = false ->
    gvar_init gv = idata ->
    tc_environ Delta rho ->
-   globvar2pred(i, gv) rho |--
-   (EX s:val, local (locald_denote (gvar i s)) && init_data_list2pred idata (readonly2share (gvar_readonly gv)) s) rho.
+   globvar2pred (globals_of_env rho)  (i, gv) rho |--
+   init_data_list2pred idata (readonly2share (gvar_readonly gv)) (globals_of_env rho i) rho.
 Proof.
 pose (H2:=True).
 pose (H4:=True).
@@ -91,12 +92,9 @@ simpl.
 destruct H6 as [? [? [? ?]]].
 destruct (H9 i _ H0); [ | destruct H10; congruence].
 destruct (H8 _ _ H0) as [b ?].
+unfold globals_of_env. 
 rewrite H11. rewrite H1.
-rewrite H3; simpl.
-apply exp_right with (Vptr b Ptrofs.zero).
-apply andp_right. apply prop_right. hnf; rewrite H11.
-unfold Map.get. rewrite H10. auto.
-auto.
+rewrite H3; simpl. auto.
 Qed.
 
 Definition zero_of_type (t: type) : val :=
@@ -138,7 +136,7 @@ contradiction.
 Qed.
 
 Definition init_data2pred' {cs: compspecs}
-     (Delta: tycontext)  (d: init_data)  (sh: share) (ty: type) (v: val) : environ -> mpred :=
+     (Delta: tycontext) (gv: globals) (d: init_data)  (sh: share) (ty: type) (v: val) : environ -> mpred :=
  match d with
   | Init_int8 i => `(mapsto sh tuchar v (Vint (Int.zero_ext 8 i)))
   | Init_int16 i => `(mapsto sh tushort v (Vint (Int.zero_ext 16 i)))
@@ -153,7 +151,7 @@ Definition init_data2pred' {cs: compspecs}
   | Init_addrof symb ofs =>
       match (var_types Delta) ! symb, (glob_types Delta) ! symb with
       | None, Some (Tarray t n' att) =>
-         EX s:val, local (locald_denote (gvar symb s)) && `(mapsto sh (Tpointer t noattr) v (offset_val (Ptrofs.unsigned ofs) s))
+         `(mapsto sh (Tpointer t noattr) v (offset_val (Ptrofs.unsigned ofs) (gv symb)))
       | None, Some Tvoid => TT
 (*
       | None, Some t => `(mapsto sh (Tpointer t noattr) v) (`(offset_val ofs) (eval_sgvar symb t))
@@ -188,8 +186,6 @@ Proof.
  admit. (* align_compatible can be FOUND inside mapsto *)
 Admitted.
 
-Search sizeof Tpointer.
-
 Lemma sizeof_Tpointer {cs: compspecs} : forall t, 
        sizeof (Tpointer t noattr) = if Archi.ptr64 then 8 else 4.
 Proof.
@@ -218,7 +214,7 @@ Lemma init_data2pred_rejigger {cs: compspecs}:
   (alignof t | Ptrofs.unsigned (Ptrofs.repr ofs)) ->
   readable_share sh ->
    init_data2pred idata sh (offset_val ofs v) rho
-    |-- init_data2pred' Delta idata sh t (offset_val ofs v) rho.
+    |-- init_data2pred' Delta (globals_of_env rho) idata sh t (offset_val ofs v) rho .
 Proof.
 intros until v.
 intros H1 HH H1' H6' H6 H7 H8 H1'' RS.
@@ -266,14 +262,14 @@ intros H1 HH H1' H6' H6 H7 H8 H1'' RS.
    assert (locald_denote (gvar i (Vptr b' Ptrofs.zero)) rho)
      by (hnf; rewrite Hv'; rewrite H15; auto).
     destruct t0; simpl; try apply TT_right; try rewrite H8; try rewrite H;
-    (apply exp_right with (Vptr b' Ptrofs.zero); apply andp_right;
+   try  (apply exp_right with (Vptr b' Ptrofs.zero); apply andp_right;
       [unfold local, lift1; apply prop_right; auto
       |      unfold offset_val; simpl; try rewrite Ptrofs.repr_unsigned, Ptrofs.add_zero_l; auto; try apply derives_refl]).
-
+  unfold globals_of_env. rewrite H15. 
   unfold mapsto. simpl. rewrite !if_true by auto.
   rewrite andb_false_r. simpl.
   apply orp_right1.
-  apply orp_left. auto.
+  apply orp_left. normalize. rewrite Ptrofs.repr_unsigned. auto.
   normalize. inv H0.
 Qed.
 
@@ -291,7 +287,7 @@ apply juicy_mem.nonidentity_Rsh.
 Qed.
 
 Lemma unpack_globvar  {cs: compspecs}:
-  forall Delta i t gv idata,
+  forall Delta gz i t gv idata,
    (var_types Delta) ! i = None ->
    (glob_types Delta) ! i = Some t ->
   (complete_legal_cosu_type (gvar_info gv) && is_aligned cenv_cs ha_env_cs la_env_cs (gvar_info gv) 0 = true)%bool ->
@@ -300,60 +296,56 @@ Lemma unpack_globvar  {cs: compspecs}:
    gvar_init gv = idata :: nil ->
    init_data_size idata <= sizeof t ->
    sizeof t <= Ptrofs.max_unsigned ->
-   local (tc_environ Delta) && globvar2pred(i, gv) |--
-       EX s: val, local (locald_denote (gvar i s)) &&
-       init_data2pred' Delta idata (Share.lub extern_retainer (readonly2share (gvar_readonly gv))) t s.
+   local (`and (tc_environ Delta) (fun rho =>gz = globals_of_env rho)) && globvar2pred gz (i, gv) |--
+       init_data2pred' Delta gz idata (Share.lub extern_retainer (readonly2share (gvar_readonly gv))) t (gz i).
 Proof.
 intros.
-go_lowerx.
+go_lowerx. subst gz.
 eapply derives_trans; [eapply tc_globalvar_sound'; try eassumption | ].
 assert (RS: forall sh', readable_share (Share.lub sh' (readonly2share (gvar_readonly gv)))).
 intros.
 apply readable_share_lub. apply readable_share_readonly2share.
 forget (readonly2share (gvar_readonly gv)) as sh.
 autorewrite with subst norm1 norm2; normalize.
-apply exp_right with x.
-autorewrite with subst norm1 norm2; normalize.
 unfold init_data_list2pred.
-simpl.
 rewrite sepcon_emp.
-destruct (tc_eval_gvar_zero _ _ _ _ H7 H H0) as [b ?].
-assert (x = offset_val 0 x).
-hnf in H8. destruct (Map.get (ve_of rho) i) as [[? ?] | ]; try contradiction.
-destruct (ge_of rho i); try contradiction. subst; reflexivity.
-rewrite H10.
- unfold eval_var in H9.
- hnf in H8. destruct (Map.get (ve_of rho) i) as [[? ?]|]; try contradiction.
- destruct (ge_of rho i); try contradiction.
+destruct (globvar_eval_var _ _ _ _ H7 H H0) as [b [? ?]].
+(*destruct (tc_eval_gvar_zero _ _ _ _ H7 H H0) as [b ?]. *)
+assert (globals_of_env rho i = offset_val 0 (globals_of_env rho i)).
+unfold globals_of_env.
+rewrite H9. reflexivity.
+rewrite H10 at 1.
  apply derives_trans with
-    (init_data2pred' Delta idata (Share.lub extern_retainer sh) t
-      (offset_val 0 x) rho).
+    (init_data2pred' Delta (globals_of_env rho) idata (Share.lub extern_retainer sh) t
+      (offset_val 0 (globals_of_env rho i)) rho).
 + rewrite andb_true_iff in H1; destruct H1.
   eapply init_data2pred_rejigger; eauto.
-   - clear H10 H8 x. inv H9.
+   - clear H9 H8. inv H10.
       split; simpl; auto.
        change Ptrofs.max_unsigned with (Ptrofs.modulus-1) in H6.
       split3; auto.
       omega. split; auto. apply la_env_cs_sound in H11; auto.
    - omega.
    - omega.
+   - unfold globals_of_env; rewrite H9. reflexivity.
    - apply Z.divide_0_r.
  +
  unfold init_data2pred'.
+  rewrite <- H10.
  destruct idata; unfold_lift;
    try (rewrite H8; simpl; rewrite Ptrofs.add_zero_l; auto);
  try apply derives_refl.
 Qed.
 
 Fixpoint id2pred_star   {cs: compspecs}
-   (Delta: tycontext) (sh: share) (t: type) (v: val) (ofs: Z) (dl: list init_data) : environ->mpred :=
+   (Delta: tycontext) (gz: globals) (sh: share) (t: type) (v: val) (ofs: Z) (dl: list init_data) : environ->mpred :=
  match dl with
- | d::dl' => init_data2pred' Delta d sh t (offset_val ofs v)
-                   * id2pred_star Delta sh t v (ofs + init_data_size d) dl'
+ | d::dl' => init_data2pred' Delta gz d sh t (offset_val ofs v)
+                   * id2pred_star Delta gz sh t v (ofs + init_data_size d) dl'
  | nil => emp
  end.
 
-Arguments id2pred_star cs Delta sh t v ofs dl rho  / .
+Arguments id2pred_star cs Delta gz sh t v ofs dl rho  / .
 
 Lemma init_data_size_pos : forall a, init_data_size a >= 0.
 Proof.
@@ -371,26 +363,26 @@ Proof.
 Qed.
 
 Lemma unpack_globvar_star  {cs: compspecs}:
-  forall Delta i gv,
+  forall Delta gz i gv,
    (var_types Delta) ! i = None ->
    (glob_types Delta) ! i = Some (gvar_info gv) ->
   (complete_legal_cosu_type (gvar_info gv) && is_aligned cenv_cs ha_env_cs la_env_cs (gvar_info gv) 0)% bool = true ->
    gvar_volatile gv = false ->
    init_data_list_size (gvar_init gv) <= sizeof (gvar_info gv) <= Ptrofs.max_unsigned ->
-   local (tc_environ Delta) && globvar2pred(i, gv) |-- 
-      EX s:val, local (locald_denote (gvar i s)) && 
-       id2pred_star Delta (Share.lub extern_retainer (readonly2share (gvar_readonly gv))) (gvar_info gv) s 0 (gvar_init gv).
+   local (`and (tc_environ Delta) (fun rho =>gz = globals_of_env rho)) && globvar2pred gz (i, gv) |-- 
+       id2pred_star Delta gz (Share.lub extern_retainer (readonly2share (gvar_readonly gv))) (gvar_info gv) (gz i) 0 (gvar_init gv).
 Proof.
 assert (H5:=true).
 intros until 4.
 remember (gvar_info gv) as t eqn:H3; symmetry in H3.
 remember (gvar_init gv) as idata eqn:H4; symmetry in H4.
 intros.
-go_lowerx.
+go_lowerx. subst gz.
 eapply derives_trans; [eapply tc_globalvar_sound'; eassumption | ].
 normalize.
   autorewrite with subst norm1 norm2; normalize.
-apply exp_right with x.  normalize.
+
+normalize.
   autorewrite with subst norm1 norm2; normalize.
 assert (RS: forall sh', readable_share (Share.lub sh' (readonly2share (gvar_readonly gv)))).
  {intros. 
@@ -401,9 +393,10 @@ forget (readonly2share (gvar_readonly gv)) as sh.
 (* destruct (tc_eval_gvar_zero _ _ _ _ H7 H H0) as [b ?]. *)
 set (ofs:=0%Z).
 assert (alignof t | Ptrofs.unsigned (Ptrofs.repr ofs)) by (subst ofs; simpl; apply Z.divide_0_r).
-hnf in H8.  destruct (Map.get (ve_of rho) i) as [[? ?]|]; try contradiction.
-destruct (ge_of rho i); try contradiction.
-assert (H10: x = offset_val ofs x) by (subst; reflexivity).
+destruct (globvar_eval_var _ _ _ _ H7 H H0) as [b [_ H9']].
+unfold globals_of_env. rewrite H9'.
+remember (Vptr b Ptrofs.zero) as x.
+assert (H10: x = offset_val ofs x) by (subst ofs x; reflexivity).
 rewrite H10 at 1.
 (*replace (eval_var i t rho) with (offset_val (Ptrofs.repr ofs) (eval_var i t rho))
     by (rewrite H8; reflexivity). *)
@@ -412,9 +405,10 @@ assert (H11: init_data_list_size idata + ofs <= sizeof t)  by (unfold ofs; omega
 assert (H12:  sizeof t <= Ptrofs.max_unsigned)  by omega.
 assert (0 <= ofs) by (unfold ofs; omega).
 clearbody ofs.
-revert ofs H9 H10 H11 H12.
+revert ofs H8 H9 H9' H11 H12.
 clear dependent gv. clear H H0 H6.
-induction idata; simpl; auto; intros. apply derives_refl.
+induction idata; simpl; auto; intros. 
+apply derives_refl.
 apply sepcon_derives.
 * rewrite andb_true_iff in H1.
   eapply init_data2pred_rejigger; destruct H1; eauto; try tauto.
@@ -428,9 +422,11 @@ rewrite offset_offset_val.
 pose proof (init_data_size_pos a).
  apply IHidata; try omega.
  rewrite Ptrofs.unsigned_repr by omega.
- rewrite Ptrofs.unsigned_repr in H9 by omega.
+ rewrite Ptrofs.unsigned_repr in H8 by omega.
  apply Z.divide_add_r; auto.
  admit. (* alignment issue *)
+auto.
+Fail idtac.
 Admitted.
 
 Lemma tc_globalvar_sound_space {cs: compspecs} :
@@ -443,7 +439,7 @@ Lemma tc_globalvar_sound_space {cs: compspecs} :
    gvar_init gv = Init_space (sizeof t) :: nil ->
    sizeof t <= Ptrofs.max_unsigned ->
    tc_environ Delta rho ->
-   (!! ((align_compatible t) (eval_var i t rho))) && globvar2pred (i, gv) rho |-- 
+   (!! ((align_compatible t) (eval_var i t rho))) && globvar2pred (globals_of_env rho) (i, gv) rho |-- 
    data_at_ (Share.lub extern_retainer (readonly2share (gvar_readonly gv))) t (eval_var i t rho).
 Proof.
 assert (H4 := true).
@@ -486,13 +482,13 @@ Definition notboolsize (sz: intsize) : Prop :=
   match sz with IBool => False | _ => True end.
 
 Lemma id2pred_star_ZnthV_Tint  {cs: compspecs} :
- forall Delta sh n (v: val) (data: list int) sz sign mdata
+ forall Delta gz sh n (v: val) (data: list int) sz sign mdata
   (NBS: notboolsize sz),
   n = Zlength mdata ->
   mdata = map (inttype2init_data sz) data ->
   !! isptr v && !! align_compatible (Tint sz sign noattr) v &&
   !! (offset_in_range (sizeof (Tint sz sign noattr) * n)) v &&
-  id2pred_star Delta sh (tarray (Tint sz sign noattr) n) v 0 mdata |--
+  id2pred_star Delta gz sh (tarray (Tint sz sign noattr) n) v 0 mdata |--
   `(data_at sh (tarray (Tint sz sign noattr) n)
            (map (Basics.compose Vint (Cop.cast_int_int sz sign)) data) v).
 Proof.
@@ -598,12 +594,12 @@ Qed.
 *)
 
 Lemma id2pred_star_ZnthV_tint  {cs: compspecs}:
- forall Delta sh n (v: val) (data: list int) mdata,
+ forall Delta gz sh n (v: val) (data: list int) mdata,
   n = Zlength mdata ->
   mdata = map Init_int32 data ->
   !! isptr v && !! align_compatible tint v &&
   !! offset_in_range (sizeof tint * n) v &&
-  id2pred_star Delta sh (tarray tint n) v 0 mdata |--
+  id2pred_star Delta gz sh (tarray tint n) v 0 mdata |--
   `(data_at sh (tarray tint n) (map Vint data) v).
 Proof. intros; apply id2pred_star_ZnthV_Tint; auto; apply Coq.Init.Logic.I.
 Qed.
@@ -617,8 +613,16 @@ destruct (ge_of rho i); try contradiction.
 subst; apply Coq.Init.Logic.I.
 Qed.
 
+Lemma offset_zero_globals_of_env: forall rho i,
+   offset_val 0 (globals_of_env rho i) = globals_of_env rho i.
+Proof.
+intros.
+unfold globals_of_env.
+destruct (ge_of rho i); simpl; auto.
+Qed.
+
 Lemma unpack_globvar_array  {cs: compspecs}:
-  forall t sz sign (data: list int)  n Delta i gv,
+  forall t sz sign (data: list int)  n Delta gz i gv,
    (var_types Delta) ! i = None ->
    (glob_types Delta) ! i = Some (gvar_info gv) ->
    gvar_info gv = tarray t n ->
@@ -628,18 +632,17 @@ Lemma unpack_globvar_array  {cs: compspecs}:
    n = Zlength (gvar_init gv) ->
    gvar_init gv = map (inttype2init_data sz) data ->
    init_data_list_size (gvar_init gv) <= sizeof (gvar_info gv) <= Ptrofs.max_unsigned ->
-   local (tc_environ Delta) && globvar2pred(i, gv) |--
-   EX s:val, local (locald_denote (gvar i s)) &&
+   local (`and (tc_environ Delta) (fun rho =>gz = globals_of_env rho)) && globvar2pred gz(i, gv) |--
       `(data_at (Share.lub extern_retainer (readonly2share (gvar_readonly gv)))
          (tarray (Tint sz sign noattr) n)
          (map (Basics.compose Vint (Cop.cast_int_int sz sign)) data)
-         s).
+         (gz i)).
 Proof.
   intros. subst t.
   match goal with |- ?A |-- _ =>
     erewrite (add_andp A (local (tc_environ Delta)))
   end.
-  2: solve [apply andp_left1; cancel].
+ 2: solve [apply andp_left1; unfold local, lift1; intro rho; apply prop_derives; intros [? ?]; auto].
   match goal with |- ?A |-- _ =>
     erewrite (add_andp A (local (`isptr (eval_var i (tarray (Tint sz sign noattr) n)))))
   end.
@@ -647,109 +650,46 @@ Proof.
     go_lowerx. apply prop_right. eapply eval_var_isptr; eauto.
     right; split; auto. rewrite <- H1; auto.
    } Unfocus.
-  eapply derives_trans;[ apply andp_derives; [ apply andp_derives; [ eapply unpack_globvar_star; try eassumption; try reflexivity | apply derives_refl]  | apply derives_refl] |].
+  eapply derives_trans.
+  apply andp_right.
+  apply andp_left1. apply andp_left1. apply andp_left1. apply derives_refl.
+   apply andp_derives; [ apply andp_derives; [ eapply unpack_globvar_star; try eassumption; try reflexivity | apply derives_refl]  | apply derives_refl].
 * rewrite andb_true_iff.
   split; rewrite H1.
   reflexivity.
   admit.
 *
   rewrite H1. (* rewrite H3.*)  rewrite H5.
-  normalize. apply exp_right with s.
-  apply andp_right. repeat apply andp_left1; auto.
+  rewrite <- andp_assoc.
+  apply andp_left1.
   eapply derives_trans; [| apply (id2pred_star_ZnthV_Tint Delta); auto].
  2: rewrite <- H5; auto.
 Opaque sizeof.
   go_lowerx.
 Transparent sizeof.
-  normalize.
- rename H8 into H19.
-  destruct (globvar_eval_var Delta rho _ _ H7 H H0) as [? [? ?]].
-  rewrite H1 in H8.
-  assert (align_compatible (Tint sz sign noattr) (eval_var i (tarray (Tint sz sign noattr) n) rho)). {
-    rewrite H8.
-    unfold align_compatible.
-    simpl.
+  normalize. clear H8. subst gz.
+  rewrite H1 in H6.
+  assert (align_compatible (Tint sz sign noattr) (globals_of_env rho i)). {
     admit.
   } 
-  assert (offset_in_range (sizeof (Tint sz sign noattr) * n)
-           (eval_var i (tarray (Tint sz sign noattr) n) rho)). {
-    rewrite H8.
+  assert (offset_in_range (sizeof (Tint sz sign noattr) * n) (globals_of_env rho i)). {
     unfold offset_in_range; simpl.
-    rewrite H1 in H6; simpl in H6.
+    rewrite H5 in H6; simpl in H6.
     pose proof initial_world.zlength_nonneg _ (gvar_init gv).
     rewrite Z.max_r in H6 by omega.
     unfold Ptrofs.max_unsigned in H6.
     pose proof init_data_list_size_pos (gvar_init gv).
-    omega.
+    admit.
   }
   apply andp_right; auto.
   apply prop_right.
-  hnf in H3;
-  destruct (Map.get (ve_of rho) i) as [[? ?]|]; try contradiction.
-  destruct ((ge_of rho) i); try contradiction.
-  subst s.
-  rewrite H8 in *.
   split3; auto.
+  admit.
 Admitted.
-
-Lemma process_globvar:
-  forall {cs: compspecs} {Espec: OracleKind} Delta P Q R (i: ident)
-          gv gvs SF c Post (idata : init_data) t,
-       (var_types Delta) ! i = None ->
-       (glob_types Delta) ! i = Some t ->
-  (complete_legal_cosu_type (gvar_info gv) && is_aligned cenv_cs ha_env_cs la_env_cs (gvar_info gv) 0)%bool = true ->
-       gvar_volatile gv = false ->
-       gvar_info gv = t ->
-       gvar_init gv = (idata::nil) ->
-       init_data_size idata <= sizeof t ->
-       sizeof t <= Ptrofs.max_unsigned ->
- (forall v: val,
-   semax Delta (PROPx P (LOCALx (gvar i v :: Q) (SEPx R))
-                       * (init_data2pred' Delta idata 
-                         (Share.lub  extern_retainer (readonly2share (gvar_readonly gv)))
-                         t v * globvars2pred gvs) * SF)
-     c Post) ->
- semax Delta (PROPx P (LOCALx Q (SEPx R))
-                      * globvars2pred ((i,gv)::gvs) * SF)
-     c Post.
-Proof.
-intros.
-eapply semax_pre.
-instantiate (1 := EX  s : val,
-           PROPx P (LOCALx (gvar i s :: Q)
-          (SEPx R)) * (init_data2pred' Delta idata
-             (Share.lub extern_retainer
-                (readonly2share (gvar_readonly gv))) t s 
-                *fold_right sepcon emp (map globvar2pred gvs)) * SF).
-unfold globvars2pred.
-change  (fold_right sepcon emp (map globvar2pred ((i, gv) :: gvs)))
- with (globvar2pred (i,gv) * fold_right sepcon emp (map globvar2pred gvs)).
-rewrite <- (sepcon_comm SF).
- rewrite <- sepcon_assoc.
-rewrite <- (sepcon_comm (fold_right _ _ _)).
- rewrite <- !sepcon_assoc.
-rewrite <- local_sepcon_assoc2.
-eapply derives_trans.
-apply sepcon_derives; [apply derives_refl | ].
-eapply unpack_globvar; try eassumption.
-normalize.
-apply exp_right with s.
-rewrite <- (sepcon_comm SF).
-rewrite ! sepcon_assoc.
-apply sepcon_derives; auto.
-rewrite <- insert_local.
-rewrite ! local_sepcon_assoc2.
-rewrite ! local_sepcon_assoc1.
-apply andp_derives; auto.
-apply sepcon_derives; auto.
-rewrite sepcon_comm; auto.
-apply extract_exists_pre.
-apply H7.
-Qed.
 
 Lemma process_globvar':
   forall {cs: compspecs} {Espec: OracleKind} Delta P Q R (i: ident)
-          gv gvs SF c Post (idata : init_data) t,
+          gz gv gvs SF c Post (idata : init_data) t,
        (var_types Delta) ! i = None ->
        (glob_types Delta) ! i = Some t ->
   (complete_legal_cosu_type (gvar_info gv) && is_aligned cenv_cs ha_env_cs la_env_cs (gvar_info gv) 0)%bool = true ->
@@ -758,63 +698,39 @@ Lemma process_globvar':
        gvar_init gv = (idata::nil) ->
        init_data_size idata <= sizeof t ->
        sizeof t <= Ptrofs.max_unsigned ->
- (forall v: val,
-   semax Delta (PROPx P (LOCALx (gvar i v :: Q) (SEPx R))
-                       * id2pred_star Delta
+  semax Delta (PROPx P (LOCALx (gvars gz::Q) (SEPx R))
+                       * id2pred_star Delta gz
                          (Share.lub  extern_retainer (readonly2share (gvar_readonly gv)))
-                         t v 0 (idata ::nil) * globvars2pred gvs * SF)
-     c Post) ->
- semax Delta (PROPx P (LOCALx Q (SEPx R))
-                      * globvars2pred ((i,gv)::gvs) * SF)
+                         t (gz i) 0 (idata ::nil) * globvars2pred gz gvs * SF)
+     c Post ->
+ semax Delta (PROPx P (LOCALx (gvars gz::Q) (SEPx R))
+                      * globvars2pred gz ((i,gv)::gvs) * SF)
      c Post.
 Proof.
 intros.
-eapply semax_pre.
-instantiate (1 := EX  s : val,
-           PROPx P (LOCALx (gvar i s :: Q)
-          (SEPx R)) * id2pred_star Delta
-                         (Share.lub  extern_retainer (readonly2share (gvar_readonly gv)))
-                         t s 0 (idata ::nil)
-                *fold_right sepcon emp (map globvar2pred gvs) * SF).
-unfold globvars2pred.
-change  (fold_right sepcon emp (map globvar2pred ((i, gv) :: gvs)))
- with (globvar2pred (i,gv) * fold_right sepcon emp (map globvar2pred gvs)).
-rewrite <- (sepcon_comm SF).
- rewrite <- sepcon_assoc.
-rewrite <- (sepcon_comm (fold_right _ _ _)).
- rewrite <- !sepcon_assoc.
-rewrite <- local_sepcon_assoc2.
-eapply derives_trans.
-apply sepcon_derives; [apply derives_refl | ].
-eapply unpack_globvar; try eassumption.
-normalize.
-apply exp_right with s.
-unfold id2pred_star.
-rewrite <- (sepcon_comm SF).
-rewrite ! sepcon_assoc.
-apply sepcon_derives; auto.
+eapply semax_pre; [ | apply H7]; clear H7.
+pose proof  (unpack_globvar Delta gz i t gv idata H H0 H1 H2 H3 H4 H5 H6).
+clear H H0 H1 H2 H3 H4 H5 H6.
 rewrite <- insert_local.
-rewrite ! local_sepcon_assoc2.
-rewrite ! local_sepcon_assoc1.
-match goal with |- ?A |-- ?B => apply derives_trans with  (!!isptr s && A) end.
-apply andp_right; auto.
-apply andp_left1; auto.
-intro rho. simpl. apply prop_derives.
-unfold gvar_denote. intro; destruct (Map.get (ve_of rho) i) as [[? ?]|]; try contradiction.
-destruct (ge_of rho i); try contradiction. subst; apply I.
-apply derives_extract_prop; intro.
-rewrite isptr_offset_val_zero; auto.
-clear H8.
-apply andp_derives; auto.
-rewrite emp_sepcon.
+forget (PROPx P (LOCALx Q (SEPx R))) as PQR.
+unfold globvars2pred.
+change (lift_S (LiftEnviron Prop)) with environ in *.
+unfold lift2.
+change  (fun rho : environ => gz = globals_of_env rho)
+  with (locald_denote (gvars gz)) in H7|-*.
+go_lowerx.
+normalize.
 apply sepcon_derives; auto.
-rewrite sepcon_comm; auto.
-apply extract_exists_pre.
+rewrite sepcon_assoc.
+apply sepcon_derives; auto.
+apply sepcon_derives; auto.
+unfold local, lift1 in H7. specialize (H7 rho). simpl in H7. rewrite prop_true_andp in H7 by (split; auto).
+rewrite offset_zero_globals_of_env.
 apply H7.
 Qed.
 
 Lemma process_globvar_array:
-  forall {cs: compspecs} {Espec: OracleKind} Delta P Q R (i: ident)
+  forall {cs: compspecs} {Espec: OracleKind} Delta gz P Q R (i: ident)
           gv gvs SF c Post (n: Z) (t: type)  (sz : intsize) (sign : signedness) (data : list int),
        (var_types Delta) ! i = None ->
        (glob_types Delta) ! i = Some (gvar_info gv) ->
@@ -826,58 +742,42 @@ Lemma process_globvar_array:
        gvar_init gv = map (inttype2init_data sz) data ->
        init_data_list_size (gvar_init gv) <= sizeof (gvar_info gv) <=
        Ptrofs.max_unsigned ->
- (forall v: val,
-   semax Delta (PROPx P (LOCALx (gvar i v :: Q)
+  semax Delta (PROPx P (LOCALx (gvars gz :: Q)
                       (SEPx ((data_at
                    (Share.lub extern_retainer (readonly2share (gvar_readonly gv)))
                    (tarray (Tint sz sign noattr) n)
-                   (map (Vint oo Cop.cast_int_int sz sign) data) v)
+                   (map (Vint oo Cop.cast_int_int sz sign) data) (gz i))
                     :: R)))
-                       * globvars2pred gvs * SF)
-     c Post) ->
- semax Delta (PROPx P (LOCALx Q (SEPx R))
-                      * globvars2pred ((i,gv)::gvs) * SF)
+                       * globvars2pred gz gvs * SF)
+     c Post ->
+ semax Delta (PROPx P (LOCALx (gvars gz :: Q) (SEPx R))
+                      * globvars2pred gz ((i,gv)::gvs) * SF)
      c Post.
 Proof.
 intros.
-eapply semax_pre.
-instantiate (1 := EX  v : val,
-           PROPx P (LOCALx (gvar i v :: Q)
-          (SEPx ((data_at
-                   (Share.lub extern_retainer (readonly2share (gvar_readonly gv)))
-                   (tarray (Tint sz sign noattr) n)
-                   (map (Vint oo Cop.cast_int_int sz sign) data) v) :: R))) * fold_right sepcon emp (map globvar2pred gvs) * SF).
-unfold globvars2pred.
-change  (fold_right sepcon emp (map globvar2pred ((i, gv) :: gvs)))
- with (globvar2pred (i,gv) * fold_right sepcon emp (map globvar2pred gvs)).
-rewrite <- (sepcon_comm SF).
- rewrite <- sepcon_assoc.
-rewrite <- (sepcon_comm (fold_right _ _ _)).
- rewrite <- !sepcon_assoc.
-rewrite <- local_sepcon_assoc2.
-eapply derives_trans.
-apply sepcon_derives; [apply derives_refl | ].
-eapply unpack_globvar_array; try eassumption.
-normalize.
-apply exp_right with s.
-rewrite <- (sepcon_comm SF).
-rewrite ! sepcon_assoc.
-apply sepcon_derives; auto.
-rewrite <- insert_local.
+eapply semax_pre; [ | apply H8]. clear H8.
+pose proof (unpack_globvar_array _ _ _ _ _ _ gz _ _ H H0 H1 H2 H3 H4 H5 H6 H7).
+clear H H0 H1 H2 H3 H4 H5 H6 H7.
+rewrite <- !insert_local.
 rewrite <- insert_SEP.
-rewrite ! local_sepcon_assoc2.
-rewrite ! local_sepcon_assoc1.
-apply andp_derives; auto.
-pull_left (PROPx P (LOCALx Q (SEPx R))).
-rewrite ! sepcon_assoc.
+forget (PROPx P (LOCALx Q (SEPx R))) as PQR.
+unfold globvars2pred.
+change (lift_S (LiftEnviron Prop)) with environ in *.
+unfold lift2.
+change  (fun rho : environ => gz = globals_of_env rho)
+  with (locald_denote (gvars gz)) in H8|-*.
+go_lowerx.
+normalize.
 apply sepcon_derives; auto.
-rewrite sepcon_comm; auto.
-apply extract_exists_pre.
-assumption.
+pull_right (PQR rho).
+apply sepcon_derives; auto.
+apply sepcon_derives; auto.
+unfold local, lift1 in H8. specialize (H8 rho). simpl in H8. rewrite prop_true_andp in H8 by (split; auto).
+apply H8.
 Qed.
 
 Lemma process_globvar_star':
-  forall {cs: compspecs} {Espec: OracleKind} Delta P Q R (i: ident)
+  forall {cs: compspecs} {Espec: OracleKind} Delta gz P Q R (i: ident)
           gv gvs SF c Post,
        (var_types Delta) ! i = None ->
        (glob_types Delta) ! i = Some (gvar_info gv) ->
@@ -885,57 +785,41 @@ Lemma process_globvar_star':
        gvar_volatile gv = false ->
        init_data_list_size (gvar_init gv) <= sizeof (gvar_info gv) <=
        Ptrofs.max_unsigned ->
- (forall s: val,
-   semax Delta (PROPx P (LOCALx (gvar i s :: Q)
+  semax Delta (PROPx P (LOCALx (gvars gz :: Q)
                       (SEPx R))
-                  * (id2pred_star Delta
+                  * (id2pred_star Delta gz
                           (Share.lub extern_retainer
                                (readonly2share (gvar_readonly gv)))
-                       (gvar_info gv) s 0 (gvar_init gv))
-             * globvars2pred gvs * SF)
-     c Post) ->
- semax Delta (PROPx P (LOCALx Q (SEPx R))
-                      * globvars2pred ((i,gv)::gvs) * SF)
+                       (gvar_info gv) (gz i) 0 (gvar_init gv))
+             * globvars2pred gz gvs * SF)
+     c Post ->
+ semax Delta (PROPx P (LOCALx (gvars gz :: Q) (SEPx R))
+                      * globvars2pred gz ((i,gv)::gvs) * SF)
      c Post.
 Proof.
 intros.
-eapply semax_pre.
-instantiate (1 := EX  s : val,
-           PROPx P (LOCALx (gvar i s :: Q)
-          (SEPx R))
-    * id2pred_star Delta
-             (Share.lub extern_retainer
-                (readonly2share (gvar_readonly gv))) (gvar_info gv) s 0
-             (gvar_init gv)
-     * fold_right sepcon emp (map globvar2pred gvs) * SF).
+eapply semax_pre; [ | apply H4]. clear H4.
+pose proof (unpack_globvar_star _ gz _ _ H H0 H1 H2 H3).
+clear H H0 H1 H2 H3.
+rewrite <- !insert_local.
+forget (PROPx P (LOCALx Q (SEPx R))) as PQR.
 unfold globvars2pred.
-change  (fold_right sepcon emp (map globvar2pred ((i, gv) :: gvs)))
- with (globvar2pred (i,gv) * fold_right sepcon emp (map globvar2pred gvs)).
-rewrite <- (sepcon_comm SF).
- rewrite <- sepcon_assoc.
-rewrite <- (sepcon_comm (fold_right _ _ _)).
- rewrite <- !sepcon_assoc.
-rewrite <- local_sepcon_assoc2.
-eapply derives_trans.
-apply sepcon_derives; [apply derives_refl | ].
-eapply unpack_globvar_star; try eassumption.
+change (lift_S (LiftEnviron Prop)) with environ in *.
+unfold lift2.
+change  (fun rho : environ => gz = globals_of_env rho)
+  with (locald_denote (gvars gz)) in H4|-*.
+go_lowerx.
 normalize.
-apply exp_right with s.
-rewrite <- (sepcon_comm SF).
-rewrite ! sepcon_assoc.
 apply sepcon_derives; auto.
-rewrite <- insert_local.
-rewrite ! local_sepcon_assoc2.
-rewrite ! local_sepcon_assoc1.
-apply andp_derives; auto.
+pull_right (PQR rho).
 apply sepcon_derives; auto.
-rewrite sepcon_comm; auto.
-apply extract_exists_pre.
-assumption.
+apply sepcon_derives; auto.
+unfold local, lift1 in H4. specialize (H4 rho). simpl in H4. rewrite prop_true_andp in H4 by (split; auto).
+apply H4.
 Qed.
 
 Lemma process_globvar_star:
-  forall {cs: compspecs} {Espec: OracleKind} Delta P Q R (i: ident)
+  forall {cs: compspecs} {Espec: OracleKind} Delta gz P Q R (i: ident)
           gv gvs SF c Post,
        (var_types Delta) ! i = None ->
        (glob_types Delta) ! i = Some (gvar_info gv) ->
@@ -943,61 +827,43 @@ Lemma process_globvar_star:
        gvar_volatile gv = false ->
        init_data_list_size (gvar_init gv) <= sizeof (gvar_info gv) <=
        Ptrofs.max_unsigned ->
- (forall s: val,
-   semax Delta (PROPx P (LOCALx (gvar i s :: Q)
+ semax Delta (PROPx P (LOCALx (gvars gz :: Q)
                       (SEPx R))
-                       * (id2pred_star Delta
+                       * (id2pred_star Delta gz
              (Share.lub extern_retainer
-                (readonly2share (gvar_readonly gv))) (gvar_info gv) s 0
+                (readonly2share (gvar_readonly gv))) (gvar_info gv) (gz i) 0
              (gvar_init gv) *
-                    globvars2pred gvs) * SF)
-     c Post) ->
- semax Delta (PROPx P (LOCALx Q (SEPx R))
-                      * globvars2pred ((i,gv)::gvs) * SF)
+                    globvars2pred gz gvs) * SF)
+     c Post ->
+ semax Delta (PROPx P (LOCALx (gvars gz :: Q) (SEPx R))
+                      * globvars2pred gz ((i,gv)::gvs) * SF)
      c Post.
 Proof.
 intros.
-eapply semax_pre.
-instantiate (1 := EX  s : val,
-           PROPx P (LOCALx (gvar i s :: Q)
-          (SEPx R)) * ((id2pred_star Delta
-             (Share.lub extern_retainer
-                (readonly2share (gvar_readonly gv))) (gvar_info gv) s 0
-             (gvar_init gv)) * fold_right sepcon emp (map globvar2pred gvs)) * SF).
+eapply semax_pre; [ | apply H4]. clear H4.
+pose proof (unpack_globvar_star _ gz _ _ H H0 H1 H2 H3).
+clear H H0 H1 H2 H3.
+rewrite <- !insert_local.
+forget (PROPx P (LOCALx Q (SEPx R))) as PQR.
 unfold globvars2pred.
-change  (fold_right sepcon emp (map globvar2pred ((i, gv) :: gvs)))
- with (globvar2pred (i,gv) * fold_right sepcon emp (map globvar2pred gvs)).
-rewrite <- local_sepcon_assoc1.
-rewrite <- sepcon_assoc.
-pull_left (globvar2pred (i, gv)).
-rewrite <- local_sepcon_assoc1.
-rewrite <- local_sepcon_assoc1.
-rewrite !sepcon_assoc.
-eapply derives_trans; [ apply sepcon_derives; [ | apply derives_refl] | ].
-eapply unpack_globvar_star; try eassumption.
-Intros s. Exists s.
-rewrite <- insert_local.
-rewrite ! local_sepcon_assoc1.
-apply andp_derives; auto.
-rewrite <- sepcon_assoc.
-pull_left (PROPx P (LOCALx Q (SEPx R))).
-rewrite ! sepcon_assoc.
-apply derives_refl.
-apply extract_exists_pre.
-assumption.
+change (lift_S (LiftEnviron Prop)) with environ in *.
+unfold lift2.
+change  (fun rho : environ => gz = globals_of_env rho)
+  with (locald_denote (gvars gz)) in H4|-*.
+go_lowerx.
+normalize.
+apply sepcon_derives; auto.
+pull_right (PQR rho).
+apply sepcon_derives; auto.
+apply sepcon_derives; auto.
+unfold local, lift1 in H4. specialize (H4 rho). simpl in H4. rewrite prop_true_andp in H4 by (split; auto).
+apply H4.
 Qed.
 
 Lemma map_instantiate:
   forall {A B} (f: A -> B) (x: A) (y: list B) z,
     y = map f z ->  f x :: y = map f (x :: z).
 Proof. intros. subst. reflexivity. Qed.
-
-Lemma main_pre_eq:
- forall prog u v, main_pre prog u v =
-  fold_right_sepcon' (map globvar2pred (prog_vars prog)).
-Proof.
-intros. rewrite fold_right_sepcon'_eq; reflexivity.
-Qed.
 
 Ltac expand_one_globvar :=
  (* given a proof goal of the form   local (tc_environ Delta) && globvar2pred (_,_) |-- ?33 *)
@@ -1021,12 +887,21 @@ first [
  ].
 
 Lemma main_pre_start:
- forall prog u v,
-   main_pre prog u v = (PROP() LOCAL() SEP())%assert * globvars2pred (prog_vars prog).
+ forall prog u gv,
+   main_pre prog u gv = (PROP() LOCAL(gvars gv) SEP())%assert * globvars2pred gv (prog_vars prog).
 Proof.
 intros.
-unfold main_pre, prog_vars, prog_vars', PROPx, LOCALx, SEPx.
+unfold main_pre.
+unfold globvars2pred,  PROPx, LOCALx, SEPx.
+unfold lift2.
+extensionality rho.
+simpl.
 normalize.
+unfold gvars_denote. unfold_lift. unfold local, lift1.
+fold (globals_of_env rho).
+apply pred_ext; intros; normalize.
+rewrite prop_true_andp by auto.
+auto.
 Qed.
 
 Ltac process_one_globvar :=
@@ -1129,13 +1004,8 @@ Qed.
 
 Ltac process_idstar :=
   match goal with
-  | |- semax _ (_ * globvars2pred ((?i,_)::_) * _) _ _ =>
-    match goal with
-    | n: name i |- _ => idtac
-    | |- _ => let n := fresh "v" i in assert (n: name i) by apply Logic.I
-    end;
-    match goal with
-    | n: name i |- _ => process_one_globvar; clear n; intro n;
+  | |- semax _ (_ * globvars2pred _ (_::_) * _) _ _ =>
+     process_one_globvar;
      match goal with |- semax _ (_ * ?A * _ * _) _ _ =>
          let p := fresh "p" in set (p:=A);
          simpl in p;
@@ -1155,15 +1025,24 @@ Ltac process_idstar :=
           end
         ];
       simple apply move_globfield_into_SEP0
-   | |- _ => idtac
+      | |- _ => idtac
     end
-   end
  end.
+
+Lemma eliminate_globvars2pred_nil: 
+ forall {cs: compspecs}{Espec: OracleKind} Delta PQR gv SF c Post,
+  semax Delta (PQR * SF) c Post ->
+  semax Delta (PQR * globvars2pred gv nil * SF) c Post.
+Proof.
+intros.
+eapply semax_pre; [ | apply H].
+go_lowerx; normalize.
+Qed.
 
 Ltac expand_main_pre :=
  rewrite main_pre_start;
  unfold prog_vars, prog_vars'; simpl globvars2pred;
  repeat  process_idstar;
- change (globvars2pred nil) with (@emp (environ->mpred) _ _);
- rewrite (sepcon_emp (PROPx _ _));
+ apply eliminate_globvars2pred_nil;
  rewrite ?offset_val_unsigned_repr.
+
