floyd/sublist.v
@@ -1610,8 +1610,8 @@ Proof.
   apply Z.max_lub_lt; omega.
 Qed.
 
-Lemma nth_Znth {A}:
-   forall n (xs:list A) (x:A) (d: Inhabitant A), 0 <= n < Zlength xs -> (nth (Z.to_nat n) xs d) = (Znth n xs).
+Lemma nth_Znth {A} {d: Inhabitant A}:
+forall n (xs:list A), 0 <= n < Zlength xs -> (nth (Z.to_nat n) xs d) = (Znth n xs).
 Proof. intros; unfold Znth; if_tac; unfold default. omega. reflexivity. Qed.
 
 
