mailbox/verif_mailbox_specs.v
@@ -324,9 +324,9 @@ Definition writer_spec :=
 
 Definition main_spec :=
  DECLARE _main
-  WITH u : unit
-  PRE  [] main_pre prog [] u
-  POST [ tint ] main_post prog [] u.
+  WITH gv: globals
+  PRE  [] main_pre prog [] gv
+  POST [ tint ] main_post prog [] gv.
 
 (* Create the environment containing all function specs. *)
 Definition Gprog : funspecs := ltac:(with_library prog [release_spec; makelock_spec; spawn_spec;
