progs/verif_global.v
@@ -5,20 +5,20 @@ Definition Vprog : varspecs.  mk_varspecs prog. Defined.
 
 Definition f_spec :=
  DECLARE _f
-  WITH g: val
+  WITH gv: globals
   PRE [  ]
           PROP  ()
-          LOCAL (gvar _g g)
-          SEP   (data_at Ews tint (Vint (Int.repr 7)) g)
+          LOCAL (gvars gv)
+          SEP   (data_at Ews tint (Vint (Int.repr 7)) (gv _g))
   POST [ tint ]
         PROP () LOCAL(temp ret_temp  (Vint (Int.repr 7)))
-           SEP (data_at Ews tint (Vint (Int.repr 7)) g).
+           SEP (data_at Ews tint (Vint (Int.repr 7)) (gv _g)).
 
 Definition main_spec :=
  DECLARE _main
-  WITH u : unit
-  PRE  [] main_pre prog [] u
-  POST [ tint ] main_post prog [] u.
+  WITH gv: globals
+  PRE  [] main_pre prog [] gv
+  POST [ tint ] main_post prog [] gv.
 
 Definition Gprog : funspecs :=
         ltac:(with_library prog [f_spec; main_spec]).
@@ -32,10 +32,9 @@ Qed.
 
 Lemma body_main:  semax_body Vprog Gprog f_main main_spec.
 Proof.
-name g _g.
 start_function.
 rewrite data_at_tuint_tint.
-forward_call g.
+forward_call gv.
 forward.
 Qed.
 
